Added files with soundness proofs

mc_reify/func_defs.v
@@ -9,7 +9,7 @@ Require Export mc_reify.bool_funcs.
 Require MirrorCore.syms.SymEnv.
 Require MirrorCore.syms.SymSum.
 Require Import MirrorCore.Subst.FMapSubst.
-Require Import MirrorCharge.RTac.ReifyLemma.
+(*Require Import MirrorCharge.RTac.ReifyLemma.*)
 Require Import floyd.proofauto.
 Require Export MirrorCore.Lambda.Expr.
 Require Export mc_reify.types.
@@ -146,6 +146,11 @@ Definition reflect ft tus tvs e (ty : typ)
  := @exprD _ _ _ (Expr_expr_fs ft) tus tvs e ty.
 
 Definition reflect_prop tbl e := reflect tbl nil nil e (typrop).
+
+Definition reflect_prop' tbl e := match (reflect tbl nil nil e typrop) with
+| Some p => p
+| None => False
+end.
 
 Definition node l o r t : expr typ func := 
 (App (App (App (Inj (inr (Data (fnode t)))) l) o) r).
