mc_reify/get_set_reif.v
@@ -2,58 +2,45 @@ Require Import  Coq.Numbers.BinNums.
 Require Import compcert.lib.Maps.
 Require Import mc_reify.func_defs.
 
+Definition DEAD : expr typ func := Inj (typ:=typ) (inr (Other fFalse)).
+
+Definition as_tree (e : expr typ func) : option
+  ((typ * expr typ func * expr typ func * expr typ func) + typ) := 
+match e with
+  | (App (App (App (Inj (inr (Data (fnode t)))) l) o) r) =>
+    Some (inl (t, l, o, r))
+  | (Inj (inr (Data (fleaf t)))) =>
+    Some (inr t)
+  | _ => None
+end.
+
 Fixpoint set_reif (i : positive) (v : expr typ func) (m : expr typ func) :  expr typ func :=
-match m with
-  | (App (App (App (Inj (inr (Data (fnode t)))) l) o) r) (* Node l o r *)=>
+match (as_tree m) with
+  | Some (inl (t,l,o,r)) (* Node l o r *)=>
     match i with 
       | xH => node l (some_reif v t) r t
       | xO ii => node (set_reif ii v l) o r t
       | xI ii => node l o (set_reif ii v r) t
     end
-  | (Inj (inr (Data (fleaf t)))) => 
+  | Some (inr t) => 
     match i with
       | xH => node (leaf t) (some_reif v t) (leaf t) t
       | xO ii => node (set_reif ii v (leaf t)) (none_reif t) (leaf t) t
       | xI ii => node (leaf t) (none_reif t) (set_reif ii v (leaf t)) t
     end
-  | _ => Inj (inr (Other fFalse))
+  | _ => DEAD
 end.
-Locate PTree.set.
-Lemma set_reif_eq :
-forall typ i v vr t tr tbl , 
-Some v = reflect tbl nil nil vr typ ->
-Some t = reflect tbl nil nil tr (typtree typ) ->
-Some (PTree.set i v t) = reflect tbl nil nil (set_reif i vr vr) (typtree typ).
-Admitted.
 
-Lemma set_reif_eq2 :
-forall typ i vr tr tbl,
-reflect tbl nil nil (App (App (Inj (inr (Data (fset typ i)))) vr) tr) (typtree typ) =
-reflect tbl nil nil (set_reif i vr tr) (typtree typ).
-Proof.
-Admitted.
 
 Fixpoint get_reif (i : positive) (m : expr typ func) :  expr typ func :=
-match m with
-  | (App (App (App (Inj (inr (Data (fnode t)))) l) o) r) (* Node l o r *)=>
+match (as_tree m) with
+  | Some (inl (t,l,o,r)) (* Node l o r *)=>
     match i with 
       | xH => some_reif o t
       | xO ii => get_reif ii l 
       | xI ii => get_reif ii r 
     end
-  | (Inj (inr (Data (fleaf t)))) => none_reif t
-  | _ => Inj (inr (Other fFalse))
+  | Some (inr t) => none_reif t
+  | _ => DEAD
 end.
 
-Lemma get_reif_eq :
-forall typ i  t tr tbl , 
-Some t = reflect tbl nil nil tr (typtree typ) ->
-Some (PTree.get i t) = reflect tbl nil nil (get_reif i tr) (tyoption typ).
-Admitted.
-
-Lemma get_reif_eq2 :
-forall typ i tr tbl,
-reflect tbl nil nil (App (Inj (inr (Data (fget typ i)))) tr) (tyoption typ) =
-reflect tbl nil nil (get_reif i tr) (tyoption typ).
-Proof.
-Admitted.
