mc_reify/reflexivity_tacs.v
@@ -3,29 +3,33 @@ Require Import MirrorCore.Lambda.ExprUnify_simul.
 Require Import MirrorCore.RTac.RTac.
 Require Import MirrorCore.Lemma.
 Require Import MirrorCore.RTac.Core.
-Require Import MirrorCharge.RTac.ReifyLemma.
+(*Require Import MirrorCharge.RTac.ReifyLemma.*)
 Require Import mc_reify.update_tycon.
-
-
-Locate SubstUpdate_ctx_subst .
 
 Existing Instance SubstUpdate_ctx_subst.
 Locate subst.
 Instance SS : SubstI.Subst subst (expr typ func) :=
   @FMapSubst.SUBST.Subst_subst _.
 
-
 Definition REFLEXIVITYTAC : rtac typ (expr typ func) :=
 fun tus tvs n m c s e => 
-match e with 
+  match e with 
 | (App (App (Inj (inr (Other (feq ty)))) l) r) =>
   match @exprUnify (ctx_subst c) typ func _ _ _ _ _ 3
-                                 tus tvs 0 s l r ty with
+                                 tus tvs 0 l r ty s with
     | Some s => RTac.Core.Solved s 
     | None =>  RTac.Core.Fail
   end
 | _ => RTac.Core.Fail
 end.
+
+Lemma REFLEXIVITYTAC_sound tbl :
+rtac_sound (Expr_expr := func_defs.Expr_expr_fs tbl) REFLEXIVITYTAC.
+unfold rtac_sound.
+intros.
+ unfold rtac_spec.
+simpl in *.
+Admitted.
 
 Definition REFLEXIVITY := REFLEXIVITYTAC.
 
