mc_reify/types.v
@@ -45,7 +45,7 @@ Inductive typ :=
 | tysum : typ -> typ -> typ
 | typrod : typ -> typ -> typ
 | tyunit
-| tylistspec : type -> ident -> typ
+(*| tylistspec : type -> ident -> typ*)
 | tyOracleKind
 | tystatement
 | tyret_assert
@@ -92,7 +92,7 @@ Fixpoint typD (t : typ) (*(m : PositiveMap.t Type)*): Type :=
         | tysum t1 t2 => sum (typD  t1 ) (typD  t2 )
         | typrod t1 t2 => prod (typD  t1 ) (typD  t2 )
         | tyunit => unit
-        | tylistspec t i => listspec t i 
+        (*| tylistspec t i => listspec t i *)
         | tyOracleKind => OracleKind
         | tystatement => statement
         | tyret_assert => ret_assert
@@ -115,6 +115,8 @@ Qed.
 
 Definition typ_eq_dec : forall a b : typ, {a = b} + {a <> b}.
   decide equality.
+Defined.
+(*
   consider (eqb_ident i i0); intros;
   try rewrite eqb_ident_spec in H. auto.
   destruct (eqb_ident_spec i i0). right. intro. intuition. subst.
@@ -124,7 +126,7 @@ Definition typ_eq_dec : forall a b : typ, {a = b} + {a <> b}.
   destruct (eqb_type_spec t t0).
   right; intuition; subst; congruence.
  Defined.
-
+*)
 
 Instance RelDec_eq_typ : RelDec (@eq typ) :=
 { rel_dec := fun a b =>
