mc_reify/get_set_reif_soundness.v
@@ -1,0 +1,89 @@
+Require Import  Coq.Numbers.BinNums.
+Require Import compcert.lib.Maps.
+Require Import mc_reify.func_defs.
+Require Import mc_reify.get_set_reif.
+
+Lemma as_tree_l : forall e t l o r,
+as_tree e = Some (inl (t, l, o, r)) ->
+e = (App (App (App (Inj (inr (Data (fnode t)))) l) o) r).
+intros.
+unfold as_tree in H.
+repeat
+match goal with 
+| [ H : match ?x with _ => _  end = _ |- _ ] => destruct x; simpl in H; try congruence end. 
+inversion H. subst. auto.
+Admitted. (*WHATEVER*)
+
+Lemma as_tree_r : forall e t,
+as_tree e = Some (inr t) ->
+e = (Inj (inr (Data (fleaf t)))).
+intros.
+unfold as_tree in H.
+repeat
+match goal with 
+| [ H : match ?x with _ => _  end = _ |- _ ] => destruct x; simpl in H; try congruence end. 
+inversion H. subst. auto.
+Admitted.
+Locate DEAD.
+Lemma set_reif_eta : forall i v m,
+  set_reif i v m =
+match (as_tree m) with
+  | Some (inl (t,l,o,r)) (* Node l o r *)=>
+    match i with 
+      | xH => node l (some_reif v t) r t
+      | xO ii => node (set_reif ii v l) o r t
+      | xI ii => node l o (set_reif ii v r) t
+    end
+  | Some (inr t) => 
+    match i with
+      | xH => node (leaf t) (some_reif v t) (leaf t) t
+      | xO ii => node (set_reif ii v (leaf t)) (none_reif t) (leaf t) t
+      | xI ii => node (leaf t) (none_reif t) (set_reif ii v (leaf t)) t
+    end
+  | _ => DEAD
+end.
+destruct i; reflexivity.
+Qed.
+
+Ltac destruct_as_tree :=
+repeat
+match goal with
+| [ H : as_tree _ = Some (inl (_ , _ , _, _)) |- _ ] => fail 1
+| [ H : as_tree _ = Some (inr _) |- _ ] => fail 1
+| [ H : as_tree _ = Some (inl (?p, _, _)) |- _ ] => destruct p
+| [ H : as_tree _ = Some (inl (?p, _)) |- _ ] => destruct p
+| [ H : as_tree _ = Some (inl ?p) |- _ ] => destruct p
+| [ H : as_tree _ = Some ?p |- _ ] => destruct p
+end.
+
+Lemma set_reif_eq :
+forall typ i v vr t tr tbl pt, 
+Some v = reflect tbl nil nil vr typ ->
+Some t = reflect tbl nil nil tr (typtree typ) ->
+reflect tbl nil nil (set_reif i vr tr) (typtree typ) = Some pt ->
+PTree.set i v t = pt.
+intros. induction i; simpl in *.
+  + destruct (as_tree tr) eqn : atr;  destruct_as_tree. 
+     - unfold reflect in *. cbv_denote in H1. 
+Locate exprD'.
+Admitted.
+
+Lemma set_reif_eq2 :
+forall typ i vr tr tbl,
+reflect tbl nil nil (App (App (Inj (inr (Data (fset typ i)))) vr) tr) (typtree typ) =
+reflect tbl nil nil (set_reif i vr tr) (typtree typ).
+Proof.
+Admitted.
+
+Lemma get_reif_eq :
+forall typ i  t tr tbl , 
+Some t = reflect tbl nil nil tr (typtree typ) ->
+Some (PTree.get i t) = reflect tbl nil nil (get_reif i tr) (tyoption typ).
+Admitted.
+
+Lemma get_reif_eq2 :
+forall typ i tr tbl,
+reflect tbl nil nil (App (Inj (inr (Data (fget typ i)))) tr) (tyoption typ) =
+reflect tbl nil nil (get_reif i tr) (tyoption typ).
+Proof.
+Admitted.
