mc_reify/symexe_soundness.v
@@ -1,0 +1,50 @@
+Require Import mc_reify.symexe.
+
+Lemma THEN_sound : forall t1 t2 tbl,
+rtac_sound (Expr_expr := func_defs.Expr_expr_fs tbl) t1 -> rtac_sound (Expr_expr := func_defs.Expr_expr_fs tbl) t2 -> rtac_sound (Expr_expr := func_defs.Expr_expr_fs tbl) (THEN t1 t2). 
+intros. unfold THEN.
+unfold THEN'. 
+apply THEN_sound; auto.
+apply runOnGoals_sound; auto;
+rtac_derive_soundness.
+apply INSTANTIATE_sound.
+apply runOnGoals_sound. auto.
+Qed.
+
+
+Lemma SYMEXE_STEP_SOUND : forall tbl, rtac_sound (Expr_expr := func_defs.Expr_expr_fs tbl) (SYMEXE_STEP tbl).
+intros. eapply AT_GOAL_sound.
+intros. destruct (get_delta_statement e);
+repeat match goal with
+         | |- context [ match ?X with _ => _ end ] =>
+           destruct X; try apply FAIL_sound
+       end.
++ unfold APPLY_SKIP.
+  generalize APPLY_sound.
+
+; eauto with typeclass_instances.
+  - apply ExprLift.vars_to_uvars_exprD'.
+  - intros. 
+    generalize (@exprUnify_sound subst typ func (RType_typ) _ (func_defs.RSym_sym tbl) _ _ _ _ _ _ _ 10).
+    unfold ExprUnify_common.unify_sound, ExprUnify_common.unify_sound_ind, LemmaApply.unify_sound.
+ admit.
+  - unfold skip_lemma. 
+    unfold lemmaD. simpl. intros. 
+    unfold ExprDsimul.ExprDenote.exprT_App.
+    simpl.
+    unfold exprT_Inj. apply semax_skip.
++ apply THEN_sound.
+  - unfold APPLY_SET'.
+    apply EAPPLY_sound; eauto with typeclass_instances.
+      * apply ExprLift.vars_to_uvars_exprD'.
+      * admit.
+      * admit. (*red. simpl.
+        unfold lemmaD'. simpl.
+        unfold exprD'_typ0. simpl. unfold ExprDsimul.ExprDenote.exprD'.
+        simpl. simpl. *)
+  - 
+        
+
+
+Lemma THEN'_sound : forall t1 t2, rtac_sound t1 -> rtac_sound t2 -> rtac_sound (THEN' t1 t2).
+
